heap_lang/lifting.v
@@ -111,6 +111,16 @@ Proof.
   intros; inv_head_step; eauto.
 Qed.
 
+Lemma wp_rec_locked E f x erec (e1 e2 : expr) Φ `{!Closed (f :b: x :b: []) erec} :
+  e1 = of_val $ locked (RecV f x erec) →
+  is_Some (to_val e2) →
+  ▷ WP subst' x e2 (subst' f e1 erec) @ E {{ Φ }} ⊢ WP App e1 e2 @ E {{ Φ }}.
+Proof.
+  intros -> [v2 ?]. unlock. rewrite -(wp_lift_pure_det_head_step' (App _ _)
+    (subst' x e2 (subst' f (Rec f x erec) erec))); eauto.
+  intros; inv_head_step; eauto.
+Qed.
+
 Lemma wp_un_op E op e v v' Φ :
   to_val e = Some v →
   un_op_eval op v = Some v' →
